WIP Tezos snapshot

code/snapshot/Tezos.fst
@@ -6,9 +6,39 @@ open FStar.HyperStack.All
 open Lib.IntTypes
 open Lib.Buffer
 
-open Hacl.Impl.Curve25519.Fields
-open Hacl.Impl.Curve25519.Generic
 
+let utils_secure_compare b1 b2 len =
+  Hacl.Utils.secure_compare b1 b2 len
+
+let curve25519_51_scalarmult shared my_priv their_pub =
+  Hacl.Curve25519_51.scalarmult shared my_priv their_pub
 
 let curve25519_51_ecdh shared my_priv their_pub =
   Hacl.Curve25519_51.ecdh shared my_priv their_pub
+
+let crypto_box_detached c tag m mlen n pk sk =
+  Hacl.NaCl.crypto_box_detached c tag m mlen n pk sk
+
+let crypto_box_open_detached m c tag mlen n pk sk =
+  Hacl.NaCl.crypto_box_open_detached m c tag mlen n pk sk
+
+let crypto_box_easy c m mlen n pk sk =
+  Hacl.NaCl.crypto_box_easy c m mlen n pk sk
+
+let crypto_box_open_easy m c clen n pk sk =
+  Hacl.NaCl.crypto_box_open_easy m c clen n pk sk
+
+let blake2b_init hash kk k nn =
+  Hacl.Blake2b.blake2b_init hash kk k nn
+
+let blake2b_update_block hash prev d =
+  Hacl.Blake2b.blake2b_update_block hash prev d
+
+let blake2b_update_last hash prev len last =
+  Hacl.Blake2b.blake2b_update_last hash prev len last
+
+let blake2b_finish output hash nn =
+  Hacl.Blake2b.blake2b_finish output hash nn
+
+let blake2b nn output ll d kk k =
+  Hacl.Blake2b.blake2b nn output ll d kk k
