code/snapshot/Tezos.fsti
@@ -2,22 +2,188 @@ module Tezos
 
 open FStar.HyperStack
 open FStar.HyperStack.All
+module ST = FStar.HyperStack.ST
 
 open Lib.IntTypes
 open Lib.Buffer
+open Lib.ByteBuffer
 
-open Hacl.Impl.Curve25519.Fields
-open Hacl.Impl.Curve25519.Generic
+module LSeq = Lib.Sequence
+module B = LowStar.Buffer
+module LBS = Lib.ByteSequence
 
-module S = Spec.Curve25519
 
-val curve25519_51_ecdh:
+val utils_secure_compare:
+    b1: buffer uint8
+  -> b2: buffer uint8
+  -> len: size_t{v len = length b1 /\ v len = length b2} ->
+  Stack bool
+    (requires fun h -> live h b1 /\ live h b2)
+    (ensures  fun h0 r h1 -> modifies0 h0 h1 /\
+    r == LBS.lbytes_eq #(v len) (B.as_seq #uint8 h0 b1) (B.as_seq #uint8 h0 b2))
+
+val curve25519_51_scalarmult:
     shared:lbuffer uint8 32ul
   -> my_priv:lbuffer uint8 32ul
-  -> their_pub:lbuffer uint8 32ul
-  -> Stack unit
+  -> their_pub:lbuffer uint8 32ul ->
+  Stack unit
     (requires fun h0 ->
       live h0 shared /\ live h0 my_priv /\ live h0 their_pub /\
       disjoint shared my_priv /\ disjoint shared their_pub)
     (ensures  fun h0 _ h1 -> modifies (loc shared) h0 h1 /\
-      as_seq h1 shared == S.scalarmult (as_seq h0 my_priv) (as_seq h0 their_pub))
+      as_seq h1 shared == Spec.Curve25519.scalarmult (as_seq h0 my_priv) (as_seq h0 their_pub))
+
+val curve25519_51_ecdh:
+    shared:lbuffer uint8 32ul
+  -> my_priv:lbuffer uint8 32ul
+  -> their_pub:lbuffer uint8 32ul ->
+  Stack bool
+    (requires fun h0 ->
+      live h0 shared /\ live h0 my_priv /\ live h0 their_pub /\
+      disjoint shared my_priv /\ disjoint shared their_pub)
+    (ensures  fun h0 r h1 -> modifies (loc shared) h0 h1 /\
+      as_seq h1 shared == Spec.Curve25519.scalarmult (as_seq h0 my_priv) (as_seq h0 their_pub)
+      /\ (not r == Lib.ByteSequence.lbytes_eq #32 (as_seq h1 shared) (Lib.Sequence.create 32 (u8 0))))
+
+// #set-options "--max_fuel 50 --max_fuel 0 --max_ifuel 0"
+
+val crypto_box_detached:
+    c:buffer uint8
+  -> tag:lbuffer uint8 16ul
+  -> m:buffer uint8
+  -> mlen:size_t{length c = v mlen /\ length m = v mlen}
+  -> n:lbuffer uint8 24ul
+  -> pk:lbuffer uint8 32ul
+  -> sk:lbuffer uint8 32ul ->
+  Stack size_t
+  (requires fun h ->
+    live h c /\ live h m /\ live h sk /\ live h pk /\ live h n /\ live h tag /\
+    disjoint tag c /\ eq_or_disjoint (m <: lbuffer uint8 mlen) (c <: lbuffer uint8 mlen) /\
+    disjoint tag m /\ disjoint n m /\ disjoint n c)
+  (ensures  fun h0 r h1 -> modifies2 c tag h0 h1 /\
+   (let tag_cipher = Spec.Box.box_detached (as_seq h0 sk) (as_seq h0 pk) (as_seq h0 n) (as_seq #MUT #uint8 #mlen h0 m) in
+    match r with
+    | 0ul -> Some? tag_cipher /\ (let (tag_s, cipher_s) = Some?.v tag_cipher in (as_seq h1 tag, as_seq #MUT #uint8 #mlen h1 c) == (tag_s, cipher_s))
+    | _ -> None? tag_cipher))
+
+val crypto_box_open_detached:
+    m:buffer uint8
+  -> c:buffer uint8
+  -> tag:lbuffer uint8 16ul
+  -> mlen:size_t{length c = v mlen /\ length m = v mlen}
+  -> n:lbuffer uint8 24ul
+  -> pk:lbuffer uint8 32ul
+  -> sk:lbuffer uint8 32ul ->
+  Stack size_t
+  (requires fun h ->
+    live h c /\ live h m /\ live h pk /\ live h sk /\ live h n /\ live h tag /\
+    disjoint tag c /\ eq_or_disjoint (m <: lbuffer uint8 mlen) (c <: lbuffer uint8 mlen) /\
+    disjoint tag m /\ disjoint n m /\ disjoint n c)
+  (ensures  fun h0 r h1 -> modifies1 m h0 h1 /\
+   (let msg = Spec.Box.box_open_detached (as_seq h0 pk) (as_seq h0 sk) (as_seq h0 n) (as_seq h0 tag) (as_seq #MUT #uint8 #mlen h0 c) in
+    match r with
+    | 0ul -> Some? msg /\ as_seq #MUT #uint8 #mlen h1 m == Some?.v msg
+    | _ -> None? msg))
+
+val crypto_box_easy:
+    c:buffer uint8
+  -> m:buffer uint8
+  -> mlen:size_t{length c = v mlen + 16 /\ length m = v mlen}
+  -> n:lbuffer uint8 24ul
+  -> pk:lbuffer uint8 32ul
+  -> sk:lbuffer uint8 32ul ->
+  Stack size_t
+  (requires fun h ->
+    live h c /\ live h m /\ live h sk /\ live h pk /\ live h n /\
+    disjoint m c /\ disjoint n m /\ disjoint n c)
+  (ensures  fun h0 r h1 -> modifies1 c h0 h1 /\
+    (let cipher = Spec.Box.box_easy (as_seq h0 sk) (as_seq h0 pk) (as_seq h0 n) (as_seq #MUT #uint8 #mlen h0 m) in
+    match r with
+    | 0ul -> Some? cipher /\ as_seq #MUT #uint8 #(mlen +! 16ul) h1 c == Some?.v cipher
+    | _ -> None? cipher))
+
+#set-options "--z3rlimit 100"
+
+val crypto_box_open_easy:
+    m:buffer uint8
+  -> c:buffer uint8
+  -> clen:size_t{length c = v clen /\ v clen = length m + 16}
+  -> n:lbuffer uint8 24ul
+  -> pk:lbuffer uint8 32ul
+  -> sk:lbuffer uint8 32ul ->
+  Stack size_t
+  (requires fun h ->
+    live h c /\ live h m /\ live h pk /\ live h sk /\ live h n /\
+    disjoint m c /\ disjoint m n /\ disjoint c n)
+  (ensures fun h0 r h1 -> modifies1 m h0 h1 /\
+   (let msg = Spec.Box.box_open_easy (as_seq h0 pk) (as_seq h0 sk) (as_seq h0 n) (as_seq #MUT #uint8 #clen h0 c) in
+    match r with
+    | 0ul -> Some? msg /\ as_seq #MUT #uint8 #(clen -! 16ul) h1 m == Some?.v msg
+    | _ -> None? msg))
+
+let hash_wp = lbuffer uint64 (size 8)
+let block_p = lbuffer uint8 (size 128)
+
+val blake2b_init:
+    hash: hash_wp
+  -> kk: size_t{v kk <= 64}
+  -> k: lbuffer uint8 kk
+  -> nn: size_t{1 <= v nn /\ v nn <= 64} ->
+  Stack unit
+    (requires (fun h -> live h hash
+                   /\ live h k
+                   /\ disjoint hash k
+                   /\ disjoint k hash))
+    (ensures  (fun h0 _ h1 -> modifies1 hash h0 h1
+                         /\ h1.[|hash|] == Spec.Blake2.blake2_init Spec.Blake2.Blake2B (v kk) h0.[|k|] (v nn)))
+
+val blake2b_update_block:
+    hash:hash_wp
+  -> prev:uint128{uint_v prev <= Spec.Blake2.max_limb Spec.Blake2.Blake2B}
+  -> d:block_p ->
+  Stack unit
+    (requires (fun h -> live h hash
+                   /\ live h d
+                   /\ disjoint hash d))
+    (ensures  (fun h0 _ h1 -> modifies1 hash h0 h1
+                         /\ h1.[|hash|] == Spec.Blake2.blake2_update_block Spec.Blake2.Blake2B (uint_v prev) h0.[|d|] h0.[|hash|]))
+
+val blake2b_update_last:
+    hash: hash_wp
+  -> prev: uint128{uint_v prev <= Spec.Blake2.max_limb Spec.Blake2.Blake2B}
+  -> len: size_t{v len <= Spec.Blake2.size_block Spec.Blake2.Blake2B}
+  -> last: lbuffer uint8 len ->
+  Stack unit
+    (requires (fun h -> live h hash
+                   /\ live h last
+                   /\ disjoint hash last))
+    (ensures  (fun h0 _ h1 -> modifies1 hash h0 h1
+                         /\ h1.[|hash|] == Spec.Blake2.blake2_update_last Spec.Blake2.Blake2B (uint_v prev) (v len) h0.[|last|] h0.[|hash|]))
+
+val blake2b_finish:
+    nn: size_t{1 <= v nn /\ v nn <= 64}
+  -> output: lbuffer uint8 nn
+  -> hash: hash_wp ->
+  Stack unit
+    (requires (fun h -> live h hash
+                   /\ live h output
+                   /\ disjoint output hash
+                   /\ disjoint hash output))
+    (ensures  (fun h0 _ h1 -> modifies1 output h0 h1
+                         /\ h1.[|output|] == Spec.Blake2.blake2_finish Spec.Blake2.Blake2B h0.[|hash|] (v nn)))
+
+val blake2b:
+    nn:size_t{1 <= v nn /\ v nn <= 64}
+  -> output: lbuffer uint8 nn
+  -> ll: size_t
+  -> d: lbuffer uint8 ll
+  -> kk: size_t{v kk <= 64 /\ (if v kk = 0 then v ll < pow2 128 else v ll + 128 < pow2 128)}
+  -> k: lbuffer uint8 kk ->
+  Stack unit
+    (requires (fun h -> live h output
+                   /\ live h d
+                   /\ live h k
+                   /\ disjoint output d
+                   /\ disjoint output k))
+    (ensures  (fun h0 _ h1 -> modifies (loc output) h0 h1
+                         /\ h1.[|output|] == Spec.Blake2.blake2b h0.[|d|] (v kk) h0.[|k|] (v nn)))
